Add customization options for auth and config

test/api/dotnet/ClientTests.cs
@@ -6,7 +6,6 @@ using System.Linq;
 using System.Text;
 using System.Threading.Tasks;
 using KeyringDefs;
-using KMSUtils;
 using Org.BouncyCastle.Security;
 using Xunit;
 
